src/opt/Reorder.v
@@ -65,11 +65,11 @@ Proof.
   ii. inv STEP_TGT; inv STEP; try (inv STATE; inv INSTR; inv REORDER); ss.
   - (* promise *)
     exploit sim_local_promise; eauto. i. des.
-    eexists _, _, _, _, _, _. splits; eauto.
+    eexists _, _, _, _, _, _, _. splits; eauto.
     econs 1. econs; eauto.
   - (* load *)
     exploit sim_local_read; eauto. i. des.
-    eexists _, _, _, _, _, _. splits; eauto.
+    eexists _, _, _, _, _, _, _. splits; eauto.
     + econs 2. econs 1; ss.
       * econs. econs.
       * apply progress_silent_step. auto.
@@ -78,14 +78,14 @@ Proof.
   - (* store *)
     exploit sim_local_write; eauto. i. des.
     inv STEP_SRC.
-    + eexists _, _, _, _, _, _. splits; eauto.
+    + eexists _, _, _, _, _, _, _. splits; eauto.
       * econs 2. econs 1; ss.
         { econs. econs. }
         { apply progress_silent_step. auto. }
       * left. eapply paco7_mon; [apply sim_store_sim_thread|]; ss.
         econs; eauto.
-    + eexists _, _, _, _, _, _. splits.
-      * econs 2; [|econs 1]. econs 2. econs 1; ss.
+    + eexists _, _, _, _, _, _, _. splits.
+      * econs 2; [|econs 1]. econs. econs 2. econs 1; ss.
         { econs. econs. }
         { apply progress_silent_step. auto. }
       * econs. econs; eauto.
@@ -99,15 +99,15 @@ Proof.
     { eapply Local.read_step_future; eauto. }
     i. des.
     inv STEP_SRC0.
-    + eexists _, _, _, _, _, _. splits; eauto.
+    + eexists _, _, _, _, _, _, _. splits; eauto.
       * econs 2. econs 1; ss.
         { econs. econs. }
         { apply progress_silent_step. auto. }
       * left. eapply paco7_mon; [apply sim_update_sim_thread|]; ss.
         econs; eauto.
     + exploit reorder_read_promise; try apply STEP_SRC; try apply x0; eauto. i. des.
-      eexists _, _, _, _, _, _. splits.
-      * econs 2; [|econs 1]. econs 2. econs 1; ss.
+      eexists _, _, _, _, _, _, _. splits.
+      * econs 2; [|econs 1]. econs. econs 2. econs 1; ss.
         { econs. econs. }
         { apply progress_silent_step. auto. }
       * econs 1. econs; eauto.
@@ -116,7 +116,7 @@ Proof.
         econs; eauto.
   - (* fence *)
     exploit sim_local_fence; eauto. i. des.
-    eexists _, _, _, _, _, _. splits; eauto.
+    eexists _, _, _, _, _, _, _. splits; eauto.
     + econs 2. econs 1; ss.
         { econs. econs. }
         { apply progress_silent_step. auto. }
